all the variants of Fix_eq i could imagine wanting

compiler/src/compiler/CustomFix.v
@@ -1,4 +1,81 @@
-Section FixPoint.
+(*Here we have maximum generality: dependent types and arbitrary equivalence relations*)
+Section GeneralFixPoint.
+
+Variable A : Type.
+Variable R : A -> A -> Prop.
+Hypothesis Rwf : well_founded R.
+Variable P : A -> Type.
+Variable F : forall x:A, (forall y:A, R y x -> P y) -> P x.
+Variable E1 : A -> A -> Prop.
+Variable E2 : forall {a1 a2}, P a1 -> P a2 -> Prop.
+
+Let Fix_F := @Fix_F A R P F.
+
+Lemma Fix_F_eq' (x:A) (r:Acc R x) :
+  F x (fun (y:A) (p:R y x) => Fix_F y (Acc_inv r p)) = Fix_F x r.
+Proof.
+  destruct r using Acc_inv_dep; auto.
+Qed.
+
+Let Fix := @Fix A R Rwf P F.
+
+Hypothesis
+  F_ext :
+  forall (x1 x2:A) (f1:forall y:A, R y x1 -> P y) (f2:forall y:A, R y x2 -> P y),
+    E1 x1 x2 ->
+    (forall (y1 y2:A) (p1:R y1 x1) (p2:R y2 x2),
+        E1 y1 y2 -> E2 (f1 y1 p1) (f2 y2 p2)) -> E2 (F x1 f1) (F x2 f2).
+
+Lemma Fix_F_inv' : forall (x1 x2:A) (r1:Acc R x1) (r2:Acc R x2),
+    E1 x1 x2 -> E2 (Fix_F x1 r1) (Fix_F x2 r2).
+Proof.
+  intro x1; induction (Rwf x1); intros x2 r1 r2.
+  rewrite <- (Fix_F_eq' x r1); rewrite <- (Fix_F_eq' x2 r2); intros.
+  apply F_ext; auto.
+Qed.
+
+Lemma Fix_eq' : forall (x1 x2:A),
+    E1 x1 x2 -> E2 (Fix x1) (F x2 (fun (y:A) (p:R y x2) => Fix y)).
+Proof.
+  intro x; unfold Fix, Wf.Fix.
+  rewrite <- Fix_F_eq'.
+  intros. apply F_ext; intros.
+  - assumption.
+  - apply Fix_F_inv'. assumption.
+Qed.
+End GeneralFixPoint.
+
+(*did jason do this already?  should explore
+  https://github.com/mit-plv/fiat/blob/master/src/Common/Wf1.v*)
+(*almost copied verbatim from the standard library*)
+(*allows for general recursion where one argument to recursive function is a function, without using funext axiom *)
+
+(*Here we have equivalence relations but no dependent types.*)
+Section NonDepFixPoint.
+
+Variable A : Type.
+Variable R : A -> A -> Prop.
+Hypothesis Rwf : well_founded R.
+Variable P : Type.
+Variable F : forall x:A, (forall y:A, R y x -> P) -> P.
+Variable E1 : A -> A -> Prop.
+Variable E2 : P -> P -> Prop.
+
+Hypothesis
+  F_ext :
+  forall (x1 x2:A) (f1:forall y:A, R y x1 -> P) (f2:forall y:A, R y x2 -> P),
+    E1 x1 x2 ->
+    (forall (y1 y2:A) (p1:R y1 x1) (p2:R y2 x2),
+        E1 y1 y2 -> E2 (f1 y1 p1) (f2 y2 p2)) -> E2 (F x1 f1) (F x2 f2).
+
+Definition Fix_eq'_nondep := Fix_eq' A R Rwf (fun _ => P) F E1 (fun _ _ => E2) F_ext.
+
+End NonDepFixPoint.
+
+(*Here we have dependent types but equivalence relations are eq.
+  Cannot simply deduce these lemmas from supposedly-general case,
+  since there's no good way of instantiating E2 to get eq.*)
+Section EqualityFixPoint.
 
 Variable A : Type.
 Variable R : A -> A -> Prop.
@@ -10,21 +87,39 @@ Hypothesis F_ext :
   (forall (x : A) (f g : forall y : A, R y x -> P y),
       (forall (y : A) (p1 p2 : R y x), f y p1 = g y p2) -> F x f = F x g).
 
-Lemma Fix_F_inv' : 
+Lemma Fix_F_inv'_eq : 
   forall (x : A) (r s : Acc R x), Fix_F P F r = Fix_F P F s.
 Proof.
   intros x. induction (Rwf x). intros r s.
   rewrite <- Fix_F_eq. rewrite <- Fix_F_eq. apply F_ext. auto.
 Qed.
 
-Lemma Fix_eq' :
+Lemma Fix_eq'_eq :
   forall x : A, Fix Rwf P F x = F x (fun (y : A) (_ : R y x) => Fix Rwf P F y).
 Proof.
   intros. unfold Fix. rewrite <- Fix_F_eq.
-  apply F_ext. intros. apply Fix_F_inv'.
+  apply F_ext. intros. apply Fix_F_inv'_eq.
 Qed.
 
-End FixPoint.
+End EqualityFixPoint.
+
+Section EqualityNonDepFixPoint.
+
+Variable A : Type.
+Variable R : A -> A -> Prop.
+Hypothesis Rwf : well_founded R.
+Variable P : Type.
+Variable F : forall x:A, (forall y:A, R y x -> P) -> P.
+
+Hypothesis F_ext :
+  (forall (x : A) (f g : forall y : A, R y x -> P),
+      (forall (y : A) (p1 p2 : R y x), f y p1 = g y p2) -> F x f = F x g).
+
+Check Fix_eq'_eq.
+Definition Fix_eq'_eq_nondep := Fix_eq'_eq A R Rwf (fun _ => P) F F_ext.
+Check Fix_eq'_eq_nondep.
+
+End EqualityNonDepFixPoint.  
 
 Check Fix_eq.
 Definition type_of_Fix_eq :=
@@ -34,132 +129,16 @@ Definition type_of_Fix_eq :=
         (forall (y : A) (p : R y x), f y p = g y p) -> F x f = F x g) ->
     forall x : A, Fix Rwf P F x = F x (fun (y : A) (_ : R y x) => Fix Rwf P F y).
 
-Check Fix_eq'.
-Definition type_of_Fix_eq' :=
+Check Fix_eq'_eq.
+Definition type_of_Fix_eq'_eq :=
   forall (A : Type) (R : A -> A -> Prop) (Rwf : well_founded R) 
-    (P : A -> Type) (F : forall x : A, (forall y : A, R y x -> P y) -> P x),
-    (forall (x : A) (f g : forall y : A, R y x -> P y),
+         (P : A -> Type) (F : forall x : A, (forall y : A, R y x -> P y) -> P x),
+       (forall (x : A) (f g : forall y : A, R y x -> P y),
         (forall (y : A) (p1 p2 : R y x), f y p1 = g y p2) -> F x f = F x g) ->
-    forall x : A, Fix Rwf P F x = F x (fun (y : A) (_ : R y x) => Fix Rwf P F y).
+       forall x : A, Fix Rwf P F x = F x (fun (y : A) (_ : R y x) => Fix Rwf P F y).
                                
-Goal type_of_Fix_eq' -> type_of_Fix_eq.
-  cbv [type_of_Fix_eq type_of_Fix_eq']. auto. Qed.
-
-
-
-
-(*did jason do this already?  should explore
-  https://github.com/mit-plv/fiat/blob/master/src/Common/Wf1.v*)
-(*almost copied verbatim from the standard library*)
-(*allows for general recursion where one argument to recursive function is a function, without using funext axiom *)
-Section FixPoint.
-
-Variable A : Type.
-Variable R : A -> A -> Prop.
-Hypothesis Rwf : well_founded R.
-Variable P : Type. (* really I want to say that P gives one type for each equivalence class
-                      of A wrt the equivalence relation E.  Not clear how to say this though.*)
-Variable F : forall x:A, (forall y:A, R y x -> P) -> P.
-Variable E1 : A -> A -> Prop.
-Variable E2 : P -> P -> Prop.
-
-(* No need to make this my own thing; should just use Fix_F and assume it's non-dependent.*)
-Fixpoint my_Fix_F (x:A) (a:Acc R x) : P :=
-  F x (fun (y:A) (h:R y x) => my_Fix_F y (Acc_inv a h)).
-
-Scheme Acc_inv_dep := Induction for Acc Sort Prop.
-
-Lemma my_Fix_F_eq (x:A) (r:Acc R x) :
-  F x (fun (y:A) (p:R y x) => my_Fix_F y (Acc_inv r p)) = my_Fix_F x r.
-Proof.
-  destruct r using Acc_inv_dep; auto.
-Qed.
-
-Definition my_Fix (x:A) := my_Fix_F x (Rwf x).
-
-(** Proof that [well_founded_induction] satisfies the fixpoint equation.
-    It requires an extra property of the functional *)
-
-Hypothesis
-  F_ext :
-  forall (x1 x2:A) (f1:forall y:A, R y x1 -> P) (f2:forall y:A, R y x2 -> P),
-    E1 x1 x2 ->
-    (forall (y1 y2:A) (p1:R y1 x1) (p2:R y2 x2),
-        E1 y1 y2 -> E2 (f1 y1 p1) (f2 y2 p2)) -> E2 (F x1 f1) (F x2 f2).
-
-Lemma my_Fix_F_inv : forall (x1 x2:A) (r1:Acc R x1) (r2:Acc R x2),
-    E1 x1 x2 -> E2 (my_Fix_F x1 r1) (my_Fix_F x2 r2).
-Proof.
-  intro x1; induction (Rwf x1); intros x2 r1 r2.
-  rewrite <- (my_Fix_F_eq x r1); rewrite <- (my_Fix_F_eq x2 r2); intros.
-  apply F_ext; auto.
-Qed.
-
-Lemma my_Fix_eq : forall (x1 x2:A),
-    E1 x1 x2 -> E2 (my_Fix x1) (F x2 (fun (y:A) (p:R y x2) => my_Fix y)).
-Proof.
-  intro x; unfold my_Fix.
-  rewrite <- my_Fix_F_eq.
-  intros. apply F_ext; intros.
-  - assumption.
-  - apply my_Fix_F_inv. assumption.
-Qed.
-
-End FixPoint.
-
-Section FixPoint.
-
-Variable A : Type.
-Variable R : A -> A -> Prop.
-Hypothesis Rwf : well_founded R.
-Variable P : A -> Type. (* really I want to say that P gives one type for each equivalence class
-                      of A wrt the equivalence relation E.  Not clear how to say this though.*)
-Variable F : forall x:A, (forall y:A, R y x -> P y) -> P x.
-Variable E1 : A -> A -> Prop.
-Variable E2 : forall a1 a2, P a1 -> P a2 -> Prop.
-
-(* No need to make this my own thing; should just use Fix_F and assume it's non-dependent.*)
-
-Fixpoint my_Fix_F' (x:A) (a:Acc R x) : P x :=
-  F x (fun (y:A) (h:R y x) => my_Fix_F' y (Acc_inv a h)).
-
-Lemma my_Fix_F_eq' (x:A) (r:Acc R x) :
-  F x (fun (y:A) (p:R y x) => my_Fix_F' y (Acc_inv r p)) = my_Fix_F' x r.
-Proof.
-  destruct r using Acc_inv_dep; auto.
-Qed.
-
-Definition my_Fix' (x:A) := my_Fix_F' x (Rwf x).
-
-(** Proof that [well_founded_induction] satisfies the fixpoint equation.
-    It requires an extra property of the functional *) Check E2.
-
-Hypothesis
-  F_ext :
-  forall (x1 x2:A) (f1:forall y:A, R y x1 -> P y) (f2:forall y:A, R y x2 -> P y),
-    E1 x1 x2 ->
-    (forall (y1 y2:A) (p1:R y1 x1) (p2:R y2 x2),
-        E1 y1 y2 -> E2 y1 y2 (f1 y1 p1) (f2 y2 p2)) -> E2 x1 x2 (F x1 f1) (F x2 f2).
-
-Lemma my_Fix_F_inv' : forall (x1 x2:A) (r1:Acc R x1) (r2:Acc R x2),
-    E1 x1 x2 -> E2 _ _ (my_Fix_F' x1 r1) (my_Fix_F' x2 r2).
-Proof.
-  intro x1; induction (Rwf x1); intros x2 r1 r2.
-  rewrite <- (my_Fix_F_eq' x r1); rewrite <- (my_Fix_F_eq' x2 r2); intros.
-  apply F_ext; auto.
-Qed.
-
-Lemma my_Fix_eq' : forall (x1 x2:A),
-    E1 x1 x2 -> E2 _ _ (my_Fix' x1) (F x2 (fun (y:A) (p:R y x2) => my_Fix' y)).
-Proof.
-  intro x; unfold my_Fix'.
-  rewrite <- my_Fix_F_eq'.
-  intros. apply F_ext; intros.
-  - assumption.
-  - apply my_Fix_F_inv'. assumption.
-Qed.
-
-End FixPoint.
+Goal type_of_Fix_eq'_eq -> type_of_Fix_eq.
+  cbv [type_of_Fix_eq type_of_Fix_eq'_eq]. auto. Qed.
 
 Require Import bedrock2.Semantics.
 Require Import compiler.FlatImp.
